@prefix : <http://example.org/> .
@prefix dbr: <https://dbpedia.org/resource/> .
@prefix dct: <http://purl.org/dc/terms/> .
@prefix foaf: <http://xmlns.com/foaf/0.1/> .
@prefix gn: <http://www.geonames.org/ontology#> .
@prefix gndo: <https://d-nb.info/standards/elementset/gnd#> .
@prefix lime: <http://www.w3.org/ns/lemon/lime#> .
@prefix nepalica: <https://nepalica.hadw-bw.de/nepal/editions/show/> .
@prefix nepalica_reg: <https://nepalica.hadw-bw.de/nepal/ontologies/viewitem/> .
@prefix ontolex: <http://www.w3.org/ns/lemon/ontolex#> .
@prefix rdfs: <http://www.w3.org/2000/01/rdf-schema#> .
@prefix schema: <http://schema.org/> .
@prefix skos: <http://www.w3.org/2004/02/skos/core#> .
@prefix geonames: <https://sws.geonames.org/> .
@prefix dbr: <https://dbpedia.org/resource/> .
@prefix wiki: <https://de.wikipedia.org/wiki/> .
@prefix viaf: <https://viaf.org/viaf/> .
@prefix gnd: <https://d-nb.info/gnd/> .
@prefix wikidata: <https://www.wikidata.org/wiki/> .
@prefix nepalica_gloss: <https://nepalica.hadw-bw.de/nepal/words/viewitem/> .
@prefix lexvo: <http://lexvo.org/id/iso639-3/> .
@prefix ontolex: <http://www.w3.org/ns/lemon/ontolex#> .


nepalica:1 a dct:Document ,
        lime:Lexicon ;
    dct:abstract "This Lāla Mohar of the king directs the various castes to pay to the jogis at the rate of anna 1 per family."@en ;
    dct:date "VS 1827 Kārttika bright 15 Saturday"@en ;
    dct:description "This is a text edition of the project 'Documents on the History of Religion and Law of Pre-modern Nepal', Heidelberg Academy of Sciences and Humanities, https://www.hadw-bw.de/nepal."@en ;
    dct:extent "fair; complete"@en ;
    dct:format "18; 16.5; cm"@en ;
    dct:hasPart "K 30544; 1"@en ;
    dct:identifier "K_0469_0009"@en ;
    dct:issued_by "Pṛthvīnārāyaṇa; the Gosain Siddha Bhagavanta Nātha"@en ;
    dct:language lexvo:en ,
        lexvo:ne ;
    dct:place "Sallyāna; Śaiva"@en ;
    dct:publisher "Bhadrakālī; card no. 10; Po. no. 15 Gu. Bam."@en ;
    dct:source "NGMPP catalogue card; Microfilmed on 18/8/1995 as NGMPP K 469/9"@en ;
    dct:subject "jogī, ānā"@en ;
    dct:title "A copy of a lālamohara from King Pṛthvīnārāyaṇa appointing Gosāī̃ Bhagavantanātha as central overseer of jogīs (VS 1827)"@en ;
    dct:type "lālamohara; copy"@en ;
    schema:created "4/6/16, 12:56 PM; 6/11/21, 11:28 AM; 12"@en ;
    lime:language "Nepali; Devanagari"@en .

nepalica:1#en000001 a ontolex:LexicalEntry ,
        ontolex:Word ;
    :followedBy nepalica:1#en000002 ;
    ontolex:canonicalForm nepalica:1#en000001_form .

nepalica:1#en000001_form a ontolex:Form ;
    ontolex:writtenRep "Extended"@en .

nepalica:1#en000002 a ontolex:LexicalEntry ,
        ontolex:Word ;
    :followedBy nepalica:1#en000003 ;
    ontolex:canonicalForm nepalica:1#en000002_form .

nepalica:1#en000002_form a ontolex:Form ;
    ontolex:writtenRep "Abstract"@en .

nepalica:1#en000003 a ontolex:LexicalEntry ,
        ontolex:Word ;
    :followedBy nepalica:1#en000004 ;
    ontolex:canonicalForm nepalica:1#en000003_form .

nepalica:1#en000003_form a ontolex:Form ;
    ontolex:writtenRep "The"@en .

nepalica:1#en000004 a skos:Concept ;
    :followedBy nepalica:1#en000005 ;
    rdfs:comment "[fr. A. ruq'a] n. an executive order, short note, missive from the highest authority. The king, the crown prince, but also queens and the Rāṇā prime ministers issued rukkās. t.t."@en ;
    skos:prefLabel "rukkā"@ne ;
    skos:related nepalica_gloss:1900 .

nepalica:1#en000005 a foaf:Person ;
    rdfs:label "Rājendra"@ne ;
    :followedBy nepalica:1#en000006 ;
    rdfs:comment "b. December 3, 1813 (VS 1870 Maṅgsīra 24); d. July 12, 1881 [July 10, 1881 according to Buyers] (VS 1938 Āṣāḍha 26); Queens: Sāmrājyalakṣmī Devī, Rājyalakṣmī Devī Offspring with Sāmrājyalakṣmī Devī: Surendra, Upendra, Devendra; with Rājyalakṣmī Devī: Raṇendra, Bīrendra; enthroned November 20, 1816 (VS 1873 Maṅgsīra 8) after the death of his father Gīrvāṇayuddha; abdicated after the Koṭ massacre May 12, 1847 (VS 1904 Vaiśākha 31) in favour of his eldest son Surendra; Regents: Queen Lalitatripurasundarī and Bhīmasena Thāpā (1816-1837); bibl.: Rājabhaṇḍārī 2002: 27–29; http://www.royalark.net/Nepal/nepal7.htm;"@ne ;
    rdfs:seeAlso nepalica_reg:140 ,
        viaf:11114849 ;
    foaf:name "Rājendra"@ne ;
    gndo:surname "Śāha"@ne .

nepalica:1#en000006 :followedBy nepalica:1#en000007 .

nepalica:1#en000007 a foaf:Person ;
    rdfs:label "ठिठुवा विष्ट"@ne ,
        "Ṭhiṭhubā Biṣṭa"@ne ;
    :followedBy nepalica:1#en000008 ;
    schema:gender schema:Male ;
    rdfs:comment "flourished: 1820 (VS 1877);  details: together with Guṃgyāla Biṣṭa and Silin Namgyāla Biṣṭa wrote a letter to Bhīmasena Thāpā asking whether they should continue their journey from Pokhara delivering a horse to the Kathmandu Valley upon hearing news about smallpox being rampant in the three cities in the valley (E_1866_0006); further literature: for his occurence in documents Pant and Pierce 1989: 28f. n 1; for the cooperation of the influential khri-thog-pa Biṣṭa family with the Gorkhālī rulers, see Dhungel 2002: 122f., 139f. n 38."@ne ;
    rdfs:seeAlso nepalica_reg:181 ;
    skos:altLabel "Ṭhiṭubā Biṣṭa" ;
    foaf:name "Ṭhiṭhubā Biṣṭa"@ne ;
    gndo:surname "Biṣṭa"@ne .

nepalica:1#en000008 :followedBy nepalica:1#en000009 .

nepalica:1#en000009 :followedBy nepalica:1#en000010 .

nepalica:1#en000010 a foaf:Person ;
    rdfs:label "ठिठुवा विष्ट"@ne ,
        "Ṭhiṭhubā Biṣṭa"@ne ;
    :followedBy nepalica:1#en000011 ;
    schema:gender schema:Male ;
    rdfs:comment "flourished: 1820 (VS 1877);  details: together with Guṃgyāla Biṣṭa and Silin Namgyāla Biṣṭa wrote a letter to Bhīmasena Thāpā asking whether they should continue their journey from Pokhara delivering a horse to the Kathmandu Valley upon hearing news about smallpox being rampant in the three cities in the valley (E_1866_0006); further literature: for his occurence in documents Pant and Pierce 1989: 28f. n 1; for the cooperation of the influential khri-thog-pa Biṣṭa family with the Gorkhālī rulers, see Dhungel 2002: 122f., 139f. n 38."@ne ;
    rdfs:seeAlso nepalica_reg:181 ;
    skos:altLabel "Ṭhiṭubā Biṣṭa" ;
    foaf:name "Ṭhiṭhubā Biṣṭa"@ne ;
    gndo:surname "Biṣṭa"@ne .

nepalica:1#en000011 :followedBy nepalica:1#en000012 .

nepalica:1#en000012 a foaf:Person ;
    rdfs:label "ठिठुवा विष्ट"@ne ,
        "Ṭhiṭhubā Biṣṭa"@ne ;
    :followedBy nepalica:1#en000013 ;
    schema:gender schema:Male ;
    rdfs:comment "flourished: 1820 (VS 1877);  details: together with Guṃgyāla Biṣṭa and Silin Namgyāla Biṣṭa wrote a letter to Bhīmasena Thāpā asking whether they should continue their journey from Pokhara delivering a horse to the Kathmandu Valley upon hearing news about smallpox being rampant in the three cities in the valley (E_1866_0006); further literature: for his occurence in documents Pant and Pierce 1989: 28f. n 1; for the cooperation of the influential khri-thog-pa Biṣṭa family with the Gorkhālī rulers, see Dhungel 2002: 122f., 139f. n 38."@ne ;
    rdfs:seeAlso nepalica_reg:181 ;
    skos:altLabel "Ṭhiṭubā Biṣṭa" ;
    foaf:name "Ṭhiṭhubā Biṣṭa"@ne ;
    gndo:surname "Biṣṭa"@ne .

nepalica:1#en000013 a ontolex:LexicalEntry ,
        ontolex:Word ;
    :followedBy nepalica:1#en000014 ;
    ontolex:canonicalForm nepalica:1#en000013_form .

nepalica:1#en000013_form a ontolex:Form ;
    ontolex:writtenRep "ciṭhi"@en .

nepalica:1#en000014 :followedBy nepalica:1#en000015 .

nepalica:1#en000015 a foaf:Person ;
    rdfs:label "Bhīmasena Thāpā"@ne ;
    :followedBy nepalica:1#en000016 ;
    schema:gender schema:Male ;
    rdfs:comment "also known as: Bhimsen Thapa; born: August 1775; died: 28 July 1839;  father: Amara Siṃha Thāpā; details: held the titles of general, kājī (appointed April 1804; M.C. Regmi 1995: 59 n. 6), prime minister (mukhtiyāra) and regent for the infant kings Girvāṇayuddha and Surendra from 1806 to 1837, later also addressed as svāmī; normdata:"@ne ;
    rdfs:seeAlso gnd:1024044661 ,
        nepalica_reg:29 ,
        viaf:53634994 ;
    foaf:name "Bhīmasena Thāpā"@ne ;
    gndo:surname "Thāpā"@ne .

nepalica:1#en000016 a gn:Feature ;
    rdfs:label "Pokhara"@ne ,
        "पोषरा"@ne ;
    :followedBy nepalica:1#en000017 ;
    gn:name "Pokhara"@ne ;
    rdfs:comment "a city in Kaski district on one of the important trading routes between China and India; formerly in the Kingdom of Kaski; now an important tourism hub of Nepal;"@en ;
    rdfs:seeAlso geonames:1282898 ,
        gnd:4046492-1 ,
        nepalica_reg:179 ,
        viaf:131375293 .

nepalica:1#en000017 a gn:Feature ;
    rdfs:label "Nepal"@ne ,
        "नेपाल"@ne ;
    :followedBy nepalica:1#en000018 ;
    gn:name "Nepal"@ne ;
    rdfs:seeAlso nepalica_reg:214 .

nepalica:1#en000018 a ontolex:LexicalEntry ,
        ontolex:Word ;
    :followedBy nepalica:1#en000019 ;
    ontolex:canonicalForm nepalica:1#en000018_form .

nepalica:1#en000018_form a ontolex:Form ;
    ontolex:writtenRep "rukkā"@en .

nepalica:1#en000019 a skos:Concept ;
    :followedBy nepalica:1#en000020 ;
    rdfs:comment "var. sirto, sīrto, sirtto, sirttā; n. tribute paid by Vassal states to the Central government (see Adhikari 1984: 356; Pant and Pierce 1989: 94; M.C. Regmi 1978: 865; M.C. Regmi 2002: 303). t.t."@en ;
    skos:prefLabel "sirto"@ne ;
    skos:related nepalica_gloss:1932 .

nepalica:1#en000020 a skos:Concept ;
    :followedBy nepalica:1#en000021 ;
    rdfs:comment "var. cākhurā; n. a certain bird, probably Chukar partridge (Alectoris chukar [Gray]), according to Turner 1931 (s.v. cākhuro): red-legged partridge [Alectoris rufa]. See commentary to DNA_0013_0070. t.t."@en ;
    skos:prefLabel "cākhurā"@ne ;
    skos:related nepalica_gloss:1849 .

nepalica:1#en000021 a ontolex:LexicalEntry ,
        ontolex:Word ;
    :followedBy nepalica:1#en000022 ;
    ontolex:canonicalForm nepalica:1#en000021_form .

nepalica:1#en000021_form a ontolex:Form ;
    ontolex:writtenRep "The"@en .

nepalica:1#en000022 a ontolex:LexicalEntry ,
        ontolex:Word ;
    :followedBy nepalica:1#en000023 ;
    ontolex:canonicalForm nepalica:1#en000022_form .

nepalica:1#en000022_form a ontolex:Form ;
    ontolex:writtenRep "document"@en .

nepalica:1#en000023 a ontolex:LexicalEntry ,
        ontolex:Word ;
    :followedBy nepalica:1#en000024 ;
    ontolex:canonicalForm nepalica:1#en000023_form .

nepalica:1#en000023_form a ontolex:Form ;
    ontolex:writtenRep "is"@en .

nepalica:1#en000024 a ontolex:LexicalEntry ,
        ontolex:Word ;
    :followedBy nepalica:1#en000025 ;
    ontolex:canonicalForm nepalica:1#en000024_form .

nepalica:1#en000024_form a ontolex:Form ;
    ontolex:writtenRep "dated"@en .

nepalica:1#en000025 a ontolex:LexicalEntry ,
        ontolex:Word ;
    :followedBy nepalica:1#en000026 ;
    ontolex:canonicalForm nepalica:1#en000025_form .

nepalica:1#en000025_form a ontolex:Form ;
    ontolex:writtenRep "Friday"@en .

nepalica:1#en000026 a ontolex:LexicalEntry ,
        ontolex:Word ;
    :followedBy nepalica:1#en000027 ;
    ontolex:canonicalForm nepalica:1#en000026_form .

nepalica:1#en000026_form a ontolex:Form ;
    ontolex:writtenRep "the"@en .

nepalica:1#en000027 a ontolex:LexicalEntry ,
        ontolex:Word ;
    :followedBy nepalica:1#en000028 ;
    ontolex:canonicalForm nepalica:1#en000027_form .

nepalica:1#en000027_form a ontolex:Form ;
    ontolex:writtenRep "1st"@en .

nepalica:1#en000028 a ontolex:LexicalEntry ,
        ontolex:Word ;
    :followedBy nepalica:1#en000029 ;
    ontolex:canonicalForm nepalica:1#en000028_form .

nepalica:1#en000028_form a ontolex:Form ;
    ontolex:writtenRep "day"@en .

nepalica:1#en000029 a ontolex:LexicalEntry ,
        ontolex:Word ;
    :followedBy nepalica:1#en000030 ;
    ontolex:canonicalForm nepalica:1#en000029_form .

nepalica:1#en000029_form a ontolex:Form ;
    ontolex:writtenRep "of"@en .

nepalica:1#en000030 a ontolex:LexicalEntry ,
        ontolex:Word ;
    :followedBy nepalica:1#en000031 ;
    ontolex:canonicalForm nepalica:1#en000030_form .

nepalica:1#en000030_form a ontolex:Form ;
    ontolex:writtenRep "the"@en .

nepalica:1#en000031 a ontolex:LexicalEntry ,
        ontolex:Word ;
    :followedBy nepalica:1#en000032 ;
    ontolex:canonicalForm nepalica:1#en000031_form .

nepalica:1#en000031_form a ontolex:Form ;
    ontolex:writtenRep "bright"@en .

nepalica:1#en000032 a ontolex:LexicalEntry ,
        ontolex:Word ;
    :followedBy nepalica:1#en000033 ;
    ontolex:canonicalForm nepalica:1#en000032_form .

nepalica:1#en000032_form a ontolex:Form ;
    ontolex:writtenRep "fortnight"@en .

nepalica:1#en000033 a ontolex:LexicalEntry ,
        ontolex:Word ;
    :followedBy nepalica:1#en000034 ;
    ontolex:canonicalForm nepalica:1#en000033_form .

nepalica:1#en000033_form a ontolex:Form ;
    ontolex:writtenRep "of"@en .

nepalica:1#en000034 a ontolex:LexicalEntry ,
        ontolex:Word ;
    :followedBy nepalica:1#en000035 ;
    ontolex:canonicalForm nepalica:1#en000034_form .

nepalica:1#en000034_form a ontolex:Form ;
    ontolex:writtenRep "Pauṣa"@en .

nepalica:1#en000035 a ontolex:LexicalEntry ,
        ontolex:Word ;
    :followedBy nepalica:1#en000036 ;
    ontolex:canonicalForm nepalica:1#en000035_form .

nepalica:1#en000035_form a ontolex:Form ;
    ontolex:writtenRep "of"@en .

nepalica:1#en000036 a ontolex:LexicalEntry ,
        ontolex:Word ;
    :followedBy nepalica:1#en000037 ;
    ontolex:canonicalForm nepalica:1#en000036_form .

nepalica:1#en000036_form a ontolex:Form ;
    ontolex:writtenRep "the"@en .

nepalica:1#en000037 a ontolex:LexicalEntry ,
        ontolex:Word ;
    :followedBy nepalica:1#en000038 ;
    ontolex:canonicalForm nepalica:1#en000037_form .

nepalica:1#en000037_form a ontolex:Form ;
    ontolex:writtenRep "Vikrama"@en .

nepalica:1#en000038 a ontolex:LexicalEntry ,
        ontolex:Word ;
    :followedBy nepalica:1#en000039 ;
    ontolex:canonicalForm nepalica:1#en000038_form .

nepalica:1#en000038_form a ontolex:Form ;
    ontolex:writtenRep "era"@en .

nepalica:1#en000039 a ontolex:LexicalEntry ,
        ontolex:Word ;
    :followedBy nepalica:1#en000040 ;
    ontolex:canonicalForm nepalica:1#en000039_form .

nepalica:1#en000039_form a ontolex:Form ;
    ontolex:writtenRep "year"@en .

nepalica:1#en000040 a dbr:Number ;
    :followedBy nepalica:1#en000041 ;
    ontolex:writtenRep "1877"@en .

nepalica:1#en000041 a dbr:Number ;
    :followedBy nepalica:1#en000042 ;
    ontolex:writtenRep "1821"@en .

nepalica:1#en000042 a ontolex:LexicalEntry ,
        ontolex:Word ;
    ontolex:canonicalForm nepalica:1#en000042_form .

nepalica:1#en000042_form a ontolex:Form ;
    ontolex:writtenRep "CE"@en .

