@prefix foaf: <http://xmlns.com/foaf/0.1/> .
@prefix gn: <http://www.geonames.org/ontology#> .
@prefix gndo: <https://d-nb.info/standards/elementset/gnd#> .
@prefix nepalica_reg: <https://nepalica.hadw-bw.de/nepal/ontologies/viewitem/> .
@prefix rdfs: <http://www.w3.org/2000/01/rdf-schema#> .
@prefix schema: <http://schema.org/> .
@prefix skos: <http://www.w3.org/2004/02/skos/core#> .
@prefix geonames: <https://sws.geonames.org/> .
@prefix dbr: <https://dbpedia.org/resource/> .
@prefix wiki: <https://de.wikipedia.org/wiki/> .
@prefix viaf: <https://viaf.org/viaf/> .
@prefix gnd: <https://d-nb.info/gnd/> .
@prefix wikidata: <https://www.wikidata.org/wiki/> .
@prefix nepalica_gloss: <https://nepalica.hadw-bw.de/nepal/words/viewitem/> .
@prefix lime: <http://www.w3.org/ns/lemon/lime#> .
@prefix lexvo: <http://lexvo.org/id/iso639-3/> .
@prefix ontolex: <http://www.w3.org/ns/lemon/ontolex#> .


nepalica:1# a gn:Feature ;
    rdfs:label ""@ne ,
        "गौडागल्‌फामा"@ne ,
        "दा"@ne ;
    gn:name ""@ne ;
    rdfs:comment "a locality west of Tansen; the word gauḍāgalphā in E_1866_0006 probably refers to this settlement (besides \"hill district office\" gauḍā or gaũḍā means, as koṭa used in the modern name, \"fortification, fortress\")"@en ,
        "a village in Myagdi district"@en ;
    rdfs:seeAlso nepalica_reg:124 ,
        nepalica_reg:180 .

nepalica:1#Bhīmasena_Thāpā a foaf:Person ;
    rdfs:label "Bhīmasena Thāpā"@ne ;
    schema:gender schema:Male ;
    rdfs:comment "also known as: Bhimsen Thapa; born: August 1775; died: 28 July 1839;  father: Amara Siṃha Thāpā; details: held the titles of general, kājī (appointed April 1804; M.C. Regmi 1995: 59 n. 6), prime minister (mukhtiyāra) and regent for the infant kings Girvāṇayuddha and Surendra from 1806 to 1837, later also addressed as svāmī; normdata:"@ne ;
    rdfs:seeAlso dbr:Bhimsen_Thapa ,
        gnd:1024044661 ,
        nepalica_reg:29 ,
        viaf:53634994 ,
        wiki:Bhimsen_Thapa ;
    foaf:name "Bhīmasena Thāpā"@ne ;
    gndo:surname "Thāpā"@ne .

nepalica:1#Guṃgyāla_Biṣṭa a foaf:Person ;
    rdfs:label "Guṃgyāla Biṣṭa"@ne ,
        "गुंग्याल विष्ट"@ne ;
    schema:gender schema:Male ;
    rdfs:comment "flourished: 1821 (VS 1877, E_1866_0006);  details: together with Ṭhiṭhubā Biṣṭa and Silin Namgyāla Biṣṭa wrote a letter to Bhīmasena Thāpā asking whether they should continue their journey from Pokhara delivering a horse to the Kathmandu Valley upon hearing news about smallpox being rampant in the three cities in the valley (E_1866_0006); further literature: Pant and Pierce 1989: 29 n. 2 (about Kunggyel Bista) and 55 n. 2 (with further references)."@ne ;
    rdfs:seeAlso nepalica_reg:183 ;
    foaf:name "Guṃgyāla Biṣṭa"@ne ;
    gndo:surname "Biṣṭa"@ne .

nepalica:1#Nepal a gn:Feature ;
    rdfs:label "Nepal"@ne ,
        "नेपाल"@ne ;
    gn:name "Nepal"@ne ;
    rdfs:seeAlso nepalica_reg:214 .

nepalica:1#Pokhara a gn:Feature ;
    rdfs:label "Pokhara"@ne ,
        "पोषरा"@ne ;
    gn:name "Pokhara"@ne ;
    rdfs:comment "a city in Kaski district on one of the important trading routes between China and India; formerly in the Kingdom of Kaski; now an important tourism hub of Nepal;"@en ;
    rdfs:seeAlso geonames:1282898 ,
        gnd:4046492-1 ,
        nepalica_reg:179 ,
        viaf:131375293 ,
        wiki:Pokhara .

nepalica:1#Rājendra a foaf:Person ;
    rdfs:label "Rājendra"@ne ;
    rdfs:comment "b. December 3, 1813 (VS 1870 Maṅgsīra 24); d. July 12, 1881 [July 10, 1881 according to Buyers] (VS 1938 Āṣāḍha 26); Queens: Sāmrājyalakṣmī Devī, Rājyalakṣmī Devī Offspring with Sāmrājyalakṣmī Devī: Surendra, Upendra, Devendra; with Rājyalakṣmī Devī: Raṇendra, Bīrendra; enthroned November 20, 1816 (VS 1873 Maṅgsīra 8) after the death of his father Gīrvāṇayuddha; abdicated after the Koṭ massacre May 12, 1847 (VS 1904 Vaiśākha 31) in favour of his eldest son Surendra; Regents: Queen Lalitatripurasundarī and Bhīmasena Thāpā (1816-1837); bibl.: Rājabhaṇḍārī 2002: 27–29; http://www.royalark.net/Nepal/nepal7.htm;"@ne ;
    rdfs:seeAlso nepalica_reg:140 ,
        viaf:11114849 ,
        wiki:Rajendra_Bikram_Shah ;
    foaf:name "Rājendra"@ne ;
    gndo:surname "Śāha"@ne .

nepalica:1#Silin_Namgyāla_Biṣṭa a foaf:Person ;
    rdfs:label "Silin Namgyāla Biṣṭa"@ne ,
        "सिलिन्नम्‌ग्याल विष्ट"@ne ;
    schema:gender schema:Male ;
    rdfs:comment "flourished: 1821 (VS 1877, E_1866_0006);  details: together with Ṭhiṭhubā Biṣṭa and Guṃgyāla Biṣṭa wrote a letter to Bhīmasena Thāpā asking whether they should continue their journey from Pokhara delivering a horse to the Kathmandu Valley upon hearing news about smallpox being rampant in the three cities in the valley (E_1866_0006)."@ne ;
    rdfs:seeAlso nepalica_reg:182 ;
    foaf:name "Silin Namgyāla Biṣṭa"@ne ;
    gndo:surname "Biṣṭa"@ne .

nepalica:1#cākhurā a skos:Concept ;
    rdfs:comment "var. cākhurā; n. a certain bird, probably Chukar partridge (Alectoris chukar [Gray]), according to Turner 1931 (s.v. cākhuro): red-legged partridge [Alectoris rufa]. See commentary to DNA_0013_0070. t.t."@en ;
    skos:prefLabel "cākhurā"@ne ;
    skos:related nepalica_gloss:1849 .

nepalica:1#rukkā a skos:Concept ;
    rdfs:comment "[fr. A. ruq'a] n. an executive order, short note, missive from the highest authority. The king, the crown prince, but also queens and the Rāṇā prime ministers issued rukkās. t.t."@en ;
    skos:prefLabel "rukkā"@ne ;
    skos:related nepalica_gloss:1900 .

nepalica:1#sirto a skos:Concept ;
    rdfs:comment "var. sirto, sīrto, sirtto, sirttā; n. tribute paid by Vassal states to the Central government (see Adhikari 1984: 356; Pant and Pierce 1989: 94; M.C. Regmi 1978: 865; M.C. Regmi 2002: 303). t.t."@en ;
    skos:prefLabel "sirto"@ne ;
    skos:related nepalica_gloss:1932 .

nepalica:1#Ṭhiṭhubā_Biṣṭa a foaf:Person ;
    rdfs:label "ठिठुवा विष्ट"@ne ,
        "Ṭhiṭhubā Biṣṭa"@ne ;
    schema:gender schema:Male ;
    rdfs:comment "flourished: 1820 (VS 1877);  details: together with Guṃgyāla Biṣṭa and Silin Namgyāla Biṣṭa wrote a letter to Bhīmasena Thāpā asking whether they should continue their journey from Pokhara delivering a horse to the Kathmandu Valley upon hearing news about smallpox being rampant in the three cities in the valley (E_1866_0006); further literature: for his occurence in documents Pant and Pierce 1989: 28f. n 1; for the cooperation of the influential khri-thog-pa Biṣṭa family with the Gorkhālī rulers, see Dhungel 2002: 122f., 139f. n 38."@ne ;
    rdfs:seeAlso nepalica_reg:181 ;
    skos:altLabel "Ṭhiṭubā Biṣṭa" ;
    foaf:name "Ṭhiṭhubā Biṣṭa"@ne ;
    gndo:surname "Biṣṭa"@ne .

