@prefix foaf: <http://xmlns.com/foaf/0.1/> .
@prefix gn: <http://www.geonames.org/ontology#> .
@prefix gndo: <https://d-nb.info/standards/elementset/gnd#> .
@prefix nepalica_reg: <https://nepalica.hadw-bw.de/nepal/ontologies/viewitem/> .
@prefix rdfs: <http://www.w3.org/2000/01/rdf-schema#> .
@prefix schema: <http://schema.org/> .
@prefix skos: <http://www.w3.org/2004/02/skos/core#> .
@prefix geonames: <https://sws.geonames.org/> .
@prefix dbr: <https://dbpedia.org/resource/> .
@prefix wiki: <https://de.wikipedia.org/wiki/> .
@prefix viaf: <https://viaf.org/viaf/> .
@prefix gnd: <https://d-nb.info/gnd/> .
@prefix wikidata: <https://www.wikidata.org/wiki/> .
@prefix nepalica_gloss: <https://nepalica.hadw-bw.de/nepal/words/viewitem/> .
@prefix lexvo: <http://lexvo.org/id/iso639-3/> .
@prefix ontolex: <http://www.w3.org/ns/lemon/ontolex#> .


nepalica:person#Baṃba_Sāha a foaf:Person ;
    rdfs:label "Baṃba Sāha"@ne ,
        "वंव साहथि"@ne ;
    schema:gender schema:Male ;
    rdfs:comment "also known as: Baṃba Śāha, Bamma Sāhī; flourished: 1802–1818;  father: Vīrabāhu Śāha; sibling: Dilip Śāha, Hastidala Śāhī, Rudravīra Śāha / Śāhī; details: held the title of cautariyā; appointed Governor (subbā) of Kumaon in 1797 (RRS 4(4): 64"@ne ;
    rdfs:seeAlso nepalica_reg:799 ;
    skos:altLabel "Bam Sāha" ;
    foaf:name "Baṃba Sāha"@ne ;
    gndo:surname "Śāha"@ne .

nepalica:person#Gīrvāṇayuddha_Vikrama_Śāha a foaf:Person ;
    rdfs:label "Gīrvāṇayuddha Vikrama Śāha"@ne ;
    rdfs:comment "born: 1 October 1797 (VS 1854 āśv 19 gate / āśv śu 11 Sunday, according to Panta VS 2023a: 50), according to Buyers 19 October; died: 20 November 1816; father: King Raṇabahādura; mother: Queen Kāntavatī; spouses: Siddhilakṣmī, Gorakṣya Rājyalakṣmī; children: Nārendra Vikrama, King Rājendra Vikrama, Satyarūpā Rājyalakṣmī Devī, Subhāgyasundarī Rājyalakṣmī Devī; details: King of Nepal (r. 8 March 1799 (VS 1855 phāl 28 gate / phāl śu 2 Friday) – 20 November 1816); his vratabandha and marriage took place in May 1808 (VS 1865 pūrvāṅga on vai 23 gate, beginning vivāha 26 gate, Panta VS 2023b: 37-39, bāṭo chekne ritual VS 1865 vai śu 15, DNA_0015_0076); normdata:"@ne ;
    rdfs:seeAlso gnd:1024019136 ,
        nepalica_reg:209 ,
        viaf:252190742 ;
    foaf:name "Gīrvāṇayuddha Vikrama Śāha"@ne ;
    gndo:surname "Śāha"@ne .

nepalica:person#Rudravīra_Sāha a foaf:Person ;
    rdfs:label "Rudravīra Sāha"@ne ,
        "रूद्रवीर साहथि"@ne ;
    schema:gender schema:Male ;
    rdfs:comment "also known as: Rudrabīra Śāha, Rudrabīra Śāhī, Rudravīra Sāha, Rudravīra Sāhī; flourished: 1802–1809;  father: Vīrabāhu Śāha; sibling: Cautariyā Bam Śāha; details: subbā of Kumaon until 1803 (VS 1860, RRC_0005_0549) sent to the western front to help his brother Hastidala Śāhī in the siege of Kangra fort in 1805 (VS 1862); appointed subbā of Salyan in 1809 (VS 1866, Regmi 1987: 146); in 1810 (VS 1867), ordered to examine (together with Jyūṃdhana Khatrī and Raghuvira Rānā) the [corresponding] documents and, if ascertained to be correct, confirm the guṭha birtās that were given by the kings of Salyan to Bhagavantanātha (Naraharinātha VS 2022: 460, see also the summary of the lālamohara in K_0469_0017 [[doc. 15]]); subbā of Jumla in 1817 (VS 1874, K_0093_0002W)."@ne ;
    rdfs:seeAlso nepalica_reg:1702 ;
    foaf:name "Rudravīra Sāha"@ne ;
    gndo:surname "Śāha / Śāhī"@ne .

nepalica:person#Rāmānanda_Bā̃ḍā a foaf:Person ;
    rdfs:label "Rāmānanda Bā̃ḍā"@ne ;
    schema:gender schema:Male ;
    rdfs:comment "also known as: Rāmānanda Bāḍā, Ramānanda Bāḍā, Rāmānanda Śākya;  flourished: 1802 (VS 1859, E_2253_0015B)–1852 (VS 1876, K_0015_0021); father: Sarvānanda (M. Śākya 2002: 66); sibling: Ghanānanda; spouse: Jayalakṣmī; children: Amṛtānanda Vandya, Sundarānanda Vandya; details: lived in Mahābuddha, Patan; leading person of the Luthāma Guṭhī related to Bungadyo, regained the overseership of the guṭhi after a legal dispute in 1802-1803; appointed head (hākima) of Nepāla Rājakīya Pustakālaya in 1852 (M. Śākya 2002: 11); further literature: M. Śākya 2002."@ne ;
    rdfs:seeAlso nepalica_reg:1411 ;
    foaf:name "Rāmānanda Bā̃ḍā"@ne ;
    gndo:surname "Bā̃ḍā"@ne .

nepalica:person#Vīrabāhu_Sāha a foaf:Person ;
    rdfs:label "Vīrabāhu Sāha"@ne ;
    schema:gender schema:Male ;
    rdfs:comment "also known as: Bīrabāhu Sāha, Vīrabāhu Sāha; flourished: ?;  father: Candrarūpa Śāha; children: Dilip Śāha, Bam Śāha, Hastidala Śāhī, Rudravīra Śāha / Śāhī."@ne ;
    rdfs:seeAlso nepalica_reg:1703 ;
    foaf:name "Vīrabāhu Sāha"@ne ;
    gndo:surname "Śāha"@ne .

nepalica:place#Kathmandu a gn:Feature ;
    rdfs:label "Kathmandu"@ne ;
    gn:name "Kathmandu"@ne ;
    rdfs:comment "also known as: Kāḍamāḍau, Kantipur, Kāṣthamaṇḍapa, Kāṭhamāḍau, Kāṭhmāḍu, Yẽ; capital of Nepal, declared capital by Pṛthvīnārāyaṇa Śāha on 21 March 1770; a district in Central Nepal, part of Bagmati Province;"@en ;
    rdfs:seeAlso dbr:testont_dbr_1232 ,
        geonames:12095484 ,
        geonames:1283240 ,
        gnd:4030036-5 ,
        nepalica_reg:26 ,
        viaf:158284130 ,
        wiki:testont_wiki_1232 ,
        wikidata:testont_wikidata_1232 .

nepalica:place#Kumaun a gn:Feature ;
    rdfs:label "Kumaun"@ne ;
    gn:name "Kumaun"@ne ;
    rdfs:comment "also Kumāu, Kumaun; a region in the Indian State of Uttarakhand; formerly an independent kingdom, under Nepalese rule from 1791–1816;"@en ;
    rdfs:seeAlso nepalica_reg:223 .

nepalica:place#Mahābuddha_Bāhāla a gn:Feature ;
    rdfs:label "Mahābuddha Bāhāla"@ne ;
    gn:name "Mahābuddha Bāhāla"@ne ;
    rdfs:comment "a city quarter (ṭola) and a Buddhist monastery in Patan."@en ;
    rdfs:seeAlso nepalica_reg:850 .

nepalica:place#Oku_Bāhāla a gn:Feature ;
    rdfs:label "Oku Bāhāla"@ne ;
    gn:name "Oku Bāhāla"@ne ;
    rdfs:comment "also known as: Śivadevasaṃskārita Rudravarṇa Mahāvihāra; one of the major Newar Buddhist monasteries in Patan and the city quarter (ṭola) surrounding it."@en ;
    rdfs:seeAlso nepalica_reg:851 .

nepalica:place#Patan a gn:Feature ;
    rdfs:label "Patan"@ne ;
    gn:name "Patan"@ne ;
    rdfs:comment "also known as Lalitpur, Lalitapura; one of the three major cities in the Kathmandu Valley; a district in Central Nepal, part of the Bagmati Province;  _Nepal."@en ;
    rdfs:seeAlso nepalica_reg:27 .

nepalica:place#Salyan a gn:Feature ;
    rdfs:label "Salyan"@ne ;
    gn:name "Salyan"@ne ;
    rdfs:comment "not to be confused with Salyan in Dhading; also known as: a) in historical documents: Salyānā, Salyāna, Sallyānā, Śalyānā etc., b) modern spellings: Sallyāna or Salyāna; details: city and region at the rim of Dang in mid-west Nepal; a district in far-Western Nepal, part of the Karnali province; during Rana rule (1885-1950) one of the 32 districts; former principality and one of the Bāīse Rājya, sometimes also listed among the Caubīsī Rājya, ruled by: - ... - Śrīkṛṣṇa Śāha (abdicated 1793); - Raṇabhīma Śāha (1793-1809); - annexed in 1809, with Rudravīra Śāha appointed as subbā (Regmi 1971; see also Bouillier 1993: 37); - Teja Bahādura Śāha (flourished 1827–47, Regmi 1974: 161–62); - Nārendra Bahādura Śāha (r. 1847–, Regmi 1974: 162–63); - Toraṇa Divyeśvarī Devī, daughter of Dhīra Śamśera Kũvara Rāṇā (r. 1871, Regmi 1974: 163); - Lakṣmīnārāyaṇa Śāha (r. 1871–72, Regmi 1974: 163); - personally controlled by Dhīra Śamśera Kũvara Rāṇā through Subbā Jayaśaṅkara Pāṇḍe in 1872 (Regmi 1974: 163); - Śamśera Bahādura Śāha (r. 1896–, Regmi 1974: 163); - abolished as rājya in 1961, but with the rāja being allowed to retain the title Rāja of Salyan on an inheritable basis (r. 1896–, Regmi 1974: 164). _Nepal;"@en ;
    rdfs:seeAlso nepalica_reg:6 .

nepalica:term#Cautariyā a skos:Concept ;
    rdfs:comment "var. cautarīyā; n. 1) in the early Shah period, a royal collateral appointed as principal officer of the state, often kings' second and third sons; 2) later a title with no specific functions attached, granted to several male descendents of the Śāha kings at a time. Cautarīyās held different higher administrative posts, like governors (cf. Adhikari 1984: 98–99; Kumar 1967: 164-165; J.C. Regmi 1981: 32–35; M.C. Regmi 1995: 42-43); descendents of different Śāha kings of earlier periods could be nominated thus. t.t."@en ;
    skos:prefLabel "Cautariyā"@ne ;
    skos:related nepalica_gloss:901 .

nepalica:term#Guṭha a skos:Concept ;
    rdfs:comment "[fr. S. goṣṭhī] var. guṭh, guthi; n. 1) a socio-religious organization that manages and finances religious and charitable functions, a trust. 2) “endowed lands or other sources of revenue for financing religious and charitable functions“ (M.R. Pant 2002: 132; cf. M.C. Regmi 1988: 267). t.t."@en ;
    skos:prefLabel "Guṭha"@ne ;
    skos:related dbr:testword_dbr_932 ,
        geonames:testword_geonames_932 ,
        gnd:testword_gnd_932 ,
        nepalica_gloss:932 ,
        viaf:testword_viaf_932 ,
        wiki:testword_wiki_932 ,
        wikidata:testword_wikidata_932 .

nepalica:term#ijārā a skos:Concept ;
    rdfs:comment "[A.] var. ījārā; n. 1) a system under which the government granted to an individual the exclusive right to collect revenue from a specified source subject to payment of a sum stipulated in advance (M.C. Regmi 2002: 299). 2) a contract for collection of revenue, exploitation of mines, etc. (M.C. Regmi 1978: 226; cf. Adhikari 1984: 349; M.C. Regmi 1978: 162). t.t."@en ;
    skos:prefLabel "ijārā"@ne ;
    skos:related nepalica_gloss:1838 .

nepalica:term#subba a skos:Concept ;
    rdfs:comment "var. subā; n. 1) governor or chief administrative officer of a province or district (cf. Kumar 1967: 168;  Krauskopff and Meyer 2000: 185; M.R. Pant 2002: 135; M.C. Regmi 1999: 137; M.C. Regmi 2002: 303). 2) civil officer ranking higher than a mukhiyā, but lower than a sardāra (Stiller 1981: 382). According to Edwards subbās were stationed at Gorkha (cf. also Michael 2012: 134) and Chitwan, “with five others being administrators in the Terai” (Edwards 1975: 106). Edwards further mentions that “men of subba rank were also assigned in the capital to the Kumari Chowk, and Kat Bhandar offices, where they were the deputies of the kaji and kapardar in charge” (ibid.). 3) headmen of the Limbu community in the far-eastern hill regions (M.C. Regmi 1978: 229; cf. also 1978: 865). t.t."@en ;
    skos:prefLabel "subba"@ne ;
    skos:related nepalica_gloss:1109 .

