@prefix foaf: <http://xmlns.com/foaf/0.1/> .
@prefix gn: <http://www.geonames.org/ontology#> .
@prefix gndo: <https://d-nb.info/standards/elementset/gnd#> .
@prefix nepalica_reg: <https://nepalica.hadw-bw.de/nepal/ontologies/viewitem/> .
@prefix rdfs: <http://www.w3.org/2000/01/rdf-schema#> .
@prefix schema: <http://schema.org/> .
@prefix skos: <http://www.w3.org/2004/02/skos/core#> .
@prefix geonames: <https://sws.geonames.org/> .
@prefix dbr: <https://dbpedia.org/resource/> .
@prefix wiki: <https://de.wikipedia.org/wiki/> .
@prefix viaf: <https://viaf.org/viaf/> .
@prefix gnd: <https://d-nb.info/gnd/> .
@prefix wikidata: <https://www.wikidata.org/wiki/> .
@prefix nepalica_gloss: <https://nepalica.hadw-bw.de/nepal/words/viewitem/> .
@prefix lime: <http://www.w3.org/ns/lemon/lime#> .
@prefix lexvo: <http://lexvo.org/id/iso639-3/> .
@prefix ontolex: <http://www.w3.org/ns/lemon/ontolex#> .


nepalica:1#Aravindanātha_Gajuryāla a foaf:Person ;
    rdfs:label "Aravindanātha Gajuryāla"@ne ,
        "अरविन्दना गजुर्यालको"@ne ;
    schema:gender schema:Male ;
    rdfs:comment "flourished: 1821–1822;  details: astrologer studying in Varanasi."@ne ;
    rdfs:seeAlso nepalica_reg:498 ;
    foaf:name "Aravindanātha Gajuryāla"@ne ;
    gndo:surname "Gajuryāla"@ne .

nepalica:1#Bhānu_Jaisī a foaf:Person ;
    rdfs:label "Bhānu Jaisī"@ne ;
    schema:gender schema:Male ;
    rdfs:comment "also known as: Bhānu Jaisī; flourished: 18th century;  father: Jamadagni of Gorkha; details: royal astrologuer under Pṛthvīnārayaṇa Śāha; built the Śrī Bhairaveśa Mahādeva temple at Nuwakot's Devīghāṭ in 1752 (VS 1809; Vajrācārya and Śreṣṭha VS 2032: 76, appendix p. inscription no. 30)."@ne ;
    rdfs:seeAlso nepalica_reg:598 ;
    foaf:name "Bhānu Jaisī"@ne ;
    gndo:surname "Arjyāla"@ne .

nepalica:1#Bhīmasena_Thāpā a foaf:Person ;
    rdfs:label "Bhīmasena Thāpā"@ne ,
        "श्रीश्रीश्रीजनरलसाहेवभीमसेनथापाकैषु"@ne ;
    schema:gender schema:Male ;
    rdfs:comment "also known as: Bhimsen Thapa; born: August 1775; died: 28 July 1839;  father: Amara Siṃha Thāpā; details: held the titles of general, kājī (appointed April 1804; M.C. Regmi 1995: 59 n. 6), prime minister (mukhtiyāra) and regent for the infant kings Girvāṇayuddha and Surendra from 1806 to 1837, later also addressed as svāmī; normdata:"@ne ;
    rdfs:seeAlso dbr:Bhimsen_Thapa ,
        gnd:1024044661 ,
        nepalica_reg:29 ,
        viaf:53634994 ,
        wiki:Bhimsen_Thapa ;
    foaf:name "Bhīmasena Thāpā"@ne ;
    gndo:surname "Thāpā"@ne .

nepalica:1#Gīrvāṇayuddha a foaf:Person ;
    rdfs:label "Gīrvāṇayuddha"@ne ;
    rdfs:comment "born: 1 October 1797 (VS 1854 āśv 19 gate / āśv śu 11 Sunday, according to Panta VS 2023a: 50), according to Buyers 19 October; died: 20 November 1816; father: King Raṇabahādura; mother: Queen Kāntavatī; spouses: Siddhilakṣmī, Gorakṣya Rājyalakṣmī; children: Nārendra Vikrama, King Rājendra Vikrama, Satyarūpā Rājyalakṣmī Devī, Subhāgyasundarī Rājyalakṣmī Devī; details: King of Nepal (r. 8 March 1799 (VS 1855 phāl 28 gate / phāl śu 2 Friday) – 20 November 1816); his vratabandha and marriage took place in May 1808 (VS 1865 pūrvāṅga on vai 23 gate, beginning vivāha 26 gate, Panta VS 2023b: 37-39, bāṭo chekne ritual VS 1865 vai śu 15, DNA_0015_0076); normdata:"@ne ;
    rdfs:seeAlso gnd:1024019136 ,
        nepalica_reg:209 ,
        viaf:252190742 ,
        wiki:Girvan_Yuddha_Bikram_Shah ;
    foaf:name "Gīrvāṇayuddha"@ne ;
    gndo:surname "Śāha"@ne .

nepalica:1#Kathmandu a gn:Feature ;
    rdfs:label "Kathmandu"@ne ;
    gn:name "Kathmandu"@ne ;
    rdfs:comment "also known as: Kāḍamāḍau, Kantipur, Kāṣthamaṇḍapa, Kāṭhamāḍau, Kāṭhmāḍu, Yẽ; capital of Nepal, declared capital by Pṛthvīnārāyaṇa Śāha on 21 March 1770; a district in Central Nepal, part of Bagmati Province;"@en ;
    rdfs:seeAlso dbr:Kathmandu ,
        geonames:12095484 ,
        geonames:1283240 ,
        gnd:4030036-5 ,
        nepalica_reg:26 ,
        viaf:158284130 ,
        wiki:Kathmandu ,
        wiki:Kathmandu_District ,
        wikidata:testont_wikidata_1232 .

nepalica:1#Kulānanda a foaf:Person ;
    rdfs:label "Kulānanda"@ne ;
    schema:gender schema:Male ;
    rdfs:comment "flourished: 18th century;  details: held the title of royal astrologer under Pṛthvīnārayaṇa Śāha; together with Bhānu Jaisī predicted that Pṛthvīnārayaṇa Śāha would conquer the Kathmandu Valley (D.R. Panta VS 2073: 11-12)."@ne ;
    rdfs:seeAlso nepalica_reg:813 ;
    foaf:name "Kulānanda"@ne ;
    gndo:surname "Jaisī"@ne .

nepalica:1#Lalitatripurasundarī a foaf:Person ;
    rdfs:label "Lalitatripurasundarī"@ne ;
    rdfs:comment "b. 1794, d. 6 April 1832 of cholera at Kathmandu; daughter of Nayana Siṃha Thāpā and Rānā Kumārī Pā̃ḍe, sister of Māthavara Siṃha Thāpā; sixth Mahārānī of King Raṇabahādura Śāha (m. 1805); regent from 25th April 1806 until her death; wrote a treatise on Rājadharma (commentary to the Mahābhārata); had the Dhārahara tower constructed usually attributed to Bhīmasena Thāpā, and the Tripureśvara Mahādeva temple at Tripureshwar, South Kathmandu; bibl.: http://www.royalark.net/Nepal/nepal6.htm;"@ne ;
    rdfs:seeAlso nepalica_reg:190 ,
        viaf:13579330 ,
        wiki:Queen_Tripurasundari_of_Nepal ;
    foaf:name "Lalitatripurasundarī"@ne ;
    gndo:surname ""@ne .

nepalica:1#Pṛthvīnārāyaṇa_Śāha a foaf:Person ;
    rdfs:label "Pṛthvīnārāyaṇa Śāha"@ne ;
    schema:gender schema:Male ;
    rdfs:comment "born: 1720 at Gorkha; died: 11 January 1775 at Devighat;  father: Narabhūpāla Śāha, king of Gorkha; spouse: Indra Kumārī Devī, Narendra Rājyalakṣmī Devī; children: Pratāpa Siṃha Śāha, Bahādura Śāha, Vilāsa Kumārī Śāha; details: king of Gorkha (r. 3 April 1743–1768); king of Nepal (r. 1768-1775); normdata:"@ne ;
    rdfs:seeAlso dbr:Prithvi_Narayan_Sha ,
        gnd:119173816 ,
        nepalica_reg:178 ,
        viaf:5735314 ,
        wiki:Prithvi_Narayan_Shah ,
        wikidata:second_priority_when_data_is_Null ;
    foaf:name "Pṛthvīnārāyaṇa Śāha"@ne ;
    gndo:surname "Śāha"@ne .

nepalica:1#Raghunātha a foaf:Person ;
    rdfs:label "Raghunātha"@ne ;
    schema:gender schema:Male ;
    rdfs:comment "flourished: 1821 (VS 1878) - 1834 (VS 1890);  details: served the royal family as purohita."@ne ;
    rdfs:seeAlso nepalica_reg:210 ;
    foaf:name "Raghunātha"@ne ;
    gndo:surname "Arjyāla"@ne .

nepalica:1#Raṇa_Bahādura a foaf:Person ;
    rdfs:label "Raṇa Bahādura"@ne ;
    schema:gender schema:Male ;
    rdfs:comment "also known as: Paramanirguṇānanda Svāmī (after his abdication in 1799);  born: 25 May 1775; died: 25 April 1806 (killed); father: King Pratāpa Siṃha; mother: Maharānī Rājendra Rājyalakṣmī Devī; spouses: Mahārānī Rājarājeśvarī Devī (married: 1789), Mahārānī Suvarṇaprabhā Devī, Mahārānī Kāntavatī Devī (married: January 1797), Mahārānī Candrāvatī Devī (married: 1804?, cf. Stiller 1993: 47 n. 12), Mahārānī Amara Rājeśvarī Devī (married: 1804?, cf. Stiller 1993: 47 n. 12), Mahārānī Lalitatripurasundarī Devī (married: 1805), Jeṭhā Nāni Sahaba/Bhitryānī Pūrṇeśvarī, Māhilā Nāni Sahaba/Bhitryānī Mahatab, Sāhilā Nāni Sahaba/Bhitryānī Lakṣmīśvarī (married: 1804), Kānchā Bhitryānī Kasi Jāla (DNA_0013_0086, K_0096_0059) (http://www.royalark.net/Nepal/nepal6.htm); children: Raṇodyota Śāha (by Mahārānī Suvarṇaprabhā Devī), Samaraśera Śāha, (by Mahārānī Suvarṇaprabhā Devī), King Gīrvāṇayuddha (by Mahārānī Kāntavatī Devī); details: King of Nepal (r. 17 November 1777–8 March 1799, abdicated in favor of his son Gīrvāṇayuddha); left Nepal for Varanasi in April 1800, returned March 1804; became mukhtiyāra on 26 February 1806 (VS 1862 phā śu 8); assassinated by this half-brother Śerabahādura Śāha on 25 April (Nepālī 2020: 74–75; Stiller 1993: 44). normadata:"@ne ;
    rdfs:seeAlso nepalica_reg:177 ,
        wiki:Rana_Bahadur_Shah ;
    foaf:name "Raṇa Bahādura"@ne ;
    gndo:surname "Śāha"@ne .

nepalica:1#Rājendra a foaf:Person ;
    rdfs:label "Rājendra"@ne ;
    rdfs:comment "b. December 3, 1813 (VS 1870 Maṅgsīra 24); d. July 12, 1881 [July 10, 1881 according to Buyers] (VS 1938 Āṣāḍha 26); Queens: Sāmrājyalakṣmī Devī, Rājyalakṣmī Devī Offspring with Sāmrājyalakṣmī Devī: Surendra, Upendra, Devendra; with Rājyalakṣmī Devī: Raṇendra, Bīrendra; enthroned November 20, 1816 (VS 1873 Maṅgsīra 8) after the death of his father Gīrvāṇayuddha; abdicated after the Koṭ massacre May 12, 1847 (VS 1904 Vaiśākha 31) in favour of his eldest son Surendra; Regents: Queen Lalitatripurasundarī and Bhīmasena Thāpā (1816-1837); bibl.: Rājabhaṇḍārī 2002: 27–29; http://www.royalark.net/Nepal/nepal7.htm;"@ne ;
    rdfs:seeAlso nepalica_reg:140 ,
        viaf:11114849 ,
        wiki:Rajendra_Bikram_Shah ;
    foaf:name "Rājendra"@ne ;
    gndo:surname "Śāha"@ne .

nepalica:1#Sarkāra a skos:Concept ;
    rdfs:comment "n. government; head of government; king; term used to refer indistinctly to the king and/or to his government (Lecomte-Tilouine 2015: 211). t.t."@en ;
    skos:prefLabel "Sarkāra"@ne ;
    skos:related nepalica_gloss:1963 .

nepalica:1#Uprānta a skos:Concept ;
    rdfs:comment "var. uprāṃta, ūprāṃnta, ūprā̃nta, prāṃta; also yathocita uprānta; conj. after that, besides, in addition to, hereafter. In earlier prose and official documents, this word marked the beginning of a text or paragraph. It has no equivalent in English (Clark 1989: 231). In some (mostly Rāṇā period?) documents, it takes the form of yathocita uprānta. t.t."@en ;
    skos:prefLabel "Uprānta"@ne ;
    skos:related nepalica_gloss:1997 .

nepalica:1#Vārāṇasī a gn:Feature ;
    rdfs:label "Vārāṇasī"@ne ,
        "वाराणसी"@ne ;
    gn:name "Vārāṇasī"@ne ;
    rdfs:comment "also known as: Benares, Banaras, Kāśī; a city and famous pilgrimage centre on the Ganges river in northern India;"@en ;
    rdfs:seeAlso gnd:4062337-3 ,
        nepalica_reg:230 ,
        viaf:168498951 ,
        wiki:Varanasi .

nepalica:1#Śrī a skos:Concept ;
    rdfs:comment "[S.] n. word of blessing, can be used as apprecatio, in which case it means 'good fortune' (Pant and Pierce 1989: 12), can be used as a prefix to names of persons and gods, in which case it means 'venerable' or 'glorious' respectively. The number of śrīs used varies, depending on context. t.t."@en ;
    skos:prefLabel "Śrī"@ne ;
    skos:related nepalica_gloss:1869 .

