@prefix foaf: <http://xmlns.com/foaf/0.1/> .
@prefix gn: <http://www.geonames.org/ontology#> .
@prefix gndo: <https://d-nb.info/standards/elementset/gnd#> .
@prefix nepalica_reg: <https://nepalica.hadw-bw.de/nepal/ontologies/viewitem/> .
@prefix rdfs: <http://www.w3.org/2000/01/rdf-schema#> .
@prefix schema: <http://schema.org/> .
@prefix skos: <http://www.w3.org/2004/02/skos/core#> .
@prefix geonames: <https://sws.geonames.org/> .
@prefix dbr: <https://dbpedia.org/resource/> .
@prefix wiki: <https://de.wikipedia.org/wiki/> .
@prefix viaf: <https://viaf.org/viaf/> .
@prefix gnd: <https://d-nb.info/gnd/> .
@prefix wikidata: <https://www.wikidata.org/wiki/> .
@prefix nepalica_gloss: <https://nepalica.hadw-bw.de/nepal/words/viewitem/> .
@prefix lime: <http://www.w3.org/ns/lemon/lime#> .
@prefix lexvo: <http://lexvo.org/id/iso639-3/> .
@prefix ontolex: <http://www.w3.org/ns/lemon/ontolex#> .


nepalica:8637#Asaṃ_Ṭol a gn:Feature ;
    rdfs:label "Asaṃ Ṭol"@ne ,
        "असंटोल्‌का"@ne ;
    gn:name "Asaṃ Ṭol"@ne ;
    rdfs:comment "also known as: Asan Ṭol, Asana Ṭola, Asaṃ; a city quarter (ṭola) in upper (thane) Kathmandu and a central market place whose prices formed a reference point for official pricing in Nepal;"@en ;
    rdfs:seeAlso dbr:Asan,Kathmandu ,
        geonames:7962207 ,
        gnd:testont_gnd_304 ,
        nepalica_reg:304 ,
        viaf:testont_viaf_304 ,
        wiki:Asan,Kathmandu ,
        wikidata:testont_wikidata_304 ;
    skos:altLabel "Asan Ṭol"@ne ,
        "Asaṃ Ṭola"@ne .

nepalica:8637#Bengal a gn:Feature ;
    rdfs:label "Bengal"@ne ;
    gn:name "Bengal"@ne ;
    rdfs:comment "a region in the Indian subcontinent, now shared between India (West Bengal) and Bangladesh;"@en ;
    rdfs:seeAlso dbr:Bengal ,
        nepalica_reg:610 ,
        wiki:Bengal .

nepalica:8637#Bhadrakālī a gn:Feature ;
    rdfs:label "Bhadrakālī"@ne ;
    gn:name "Bhadrakālī"@ne ;
    rdfs:comment "an open air shrine (pīṭha) of the goddess Bhadrakālī east of Ṭuṇḍikhela, Kathmandu, and the area surrounding it."@en ;
    rdfs:seeAlso nepalica_reg:565 .

nepalica:8637#Bhaguṣula a gn:Feature ;
    rdfs:label "Bhaguṣula"@ne ,
        "भगुषुलको"@ne ;
    gn:name "Bhaguṣula"@ne ;
    rdfs:comment "location needs to be verified; document suggests a locality in the Kathmandu Valley."@en ;
    rdfs:seeAlso nepalica_reg:1237 ;
    skos:altLabel "Bhaguṣolā"@ne .

nepalica:8637#Bharapuranātha a foaf:Person ;
    rdfs:label "Bharapuranātha"@ne ;
    schema:gender schema:Male ;
    rdfs:comment "also known as: Bharapūranātha, Bharapuranātha Jogī, Bharpurnāthajī; born: 1880 (VS 1937/38) at the Jvālājīmaṭha in Dailekh (K_0252_0022);  father: Lachīmananātha; details: succeeded Paramahaṃsanātha as abbot (pīramahanta) of Mṛgasthalī in 1921 (VS 1978, K_0252_0018 – K_0252_0022); grandson of Uttamanātha (K_0177_0017)."@ne ;
    rdfs:seeAlso nepalica_reg:548 ;
    foaf:name "Bharapuranātha"@ne ;
    gndo:surname "Nātha"@ne .

nepalica:8637#Bhaṃgal a gn:Feature ;
    rdfs:label "Bhaṃgal"@ne ,
        "भंगल्‌को"@ne ;
    gn:name "Bhaṃgal"@ne ;
    rdfs:comment "location needs to be verified; document suggests a locality in the Kathmandu Valley."@en ;
    rdfs:seeAlso nepalica_reg:1221 ;
    skos:altLabel "Maṃgal"@ne .

nepalica:8637#Bhānumatī a foaf:Person ;
    rdfs:label "Bhānumatī"@ne ;
    schema:gender schema:Female ;
    rdfs:comment "flourished: 17th century;  spouse: King Siddhinarasiṃha Malla of Patan; children: King Śrīnivāsa Malla of Patan; details: in her name King Śrīnivāsa Malla financed a \"jogīcakraguthi\" at the Rāto Machindranātha temple at Ta Bahāla, Patan (NHDP_0001_0138) in 1673 (NS 793)."@ne ;
    rdfs:seeAlso nepalica_reg:555 ;
    foaf:name "Bhānumatī"@ne ;
    gndo:surname "Malla"@ne .

nepalica:8637#Buṅga a gn:Feature ;
    rdfs:label "Buṅga"@ne ;
    gn:name "Buṅga"@ne ;
    rdfs:comment "also Buṅga; small Newar town near Patan"@en ;
    rdfs:seeAlso nepalica_reg:553 .

nepalica:8637#Caṣu a gn:Feature ;
    rdfs:label "Caṣu"@ne ,
        "चषुछेउको"@ne ;
    gn:name "Caṣu"@ne ;
    rdfs:comment "location needs to be verified; document suggests a locality in the Kathmandu Valley."@en ;
    rdfs:seeAlso nepalica_reg:1242 .

nepalica:8637#Dalakāpa a gn:Feature ;
    rdfs:label "Dalakāpa"@ne ,
        "दलकापको"@ne ;
    gn:name "Dalakāpa"@ne ;
    rdfs:comment "also known as Dalakāpa; a locality in Kabhresthali, Kathmandu district; https://www.mindat.org/feature-7962135.html, https://nepal.places-in-the-world.com/7962135-place-dalkap.html."@en ;
    rdfs:seeAlso nepalica_reg:1216 .

nepalica:8637#Deupāṭhaṃ a gn:Feature ;
    rdfs:label "Deupāṭhaṃ"@ne ,
        "देउपाटंछेउको"@ne ;
    gn:name "Deupāṭhaṃ"@ne ;
    rdfs:comment "also known as: Deupāṭaṃ, Deupāṭana, Deūpāṭaṃ; historic town in the Kathmandu Valley, now part of Kathmandu;"@en ;
    rdfs:seeAlso gnd:4354945-7 ,
        nepalica_reg:28 ;
    skos:altLabel "Deopatan"@ne ,
        "Deupāṭan"@ne ,
        "Deupāṭaṃ"@ne .

nepalica:8637#Deurālī a gn:Feature ;
    rdfs:label "Deurālī"@ne ,
        "देउरालीमाहा"@ne ;
    gn:name "Deurālī"@ne ;
    rdfs:comment "also Deurālī; a village in Kaski district"@en ;
    rdfs:seeAlso nepalica_reg:520 ;
    skos:altLabel "Deurāli"@ne .

nepalica:8637#Dharaṃthalī a gn:Feature ;
    rdfs:label "Dharaṃthalī"@ne ,
        "धरंथलीछेउको"@ne ;
    gn:name "Dharaṃthalī"@ne ;
    rdfs:comment "also known as Dharaṃthalī, Dharmathalī; a village and former village development committee in Kathmandu district, north west of Kathmandu;"@en ;
    rdfs:seeAlso dbr:Dharmasthali ,
        nepalica_reg:519 ,
        wiki:Dharmasthali ;
    skos:altLabel "Dharaṃthali"@ne .

nepalica:8637#Dhārīnātha a foaf:Person ;
    rdfs:label "Dhārīnātha"@ne ,
        "धारीनातजी"@ne ;
    schema:gender schema:Male ;
    rdfs:comment "also known as: Dhārīnātha; flourished: 1905 (VS 1962)–1916;  details: a nāthayogī; appointed as abbot (pīramahanta) of the monastery of Gorakhanātha at Mṛgasthalī by Premier Candra Samśera in 1905 (VS 1962, K_0283_0035; cf. also K_0044_0067G; K_0441_0021); head of the Jogi Cakra Guṭhī (cf. K_0054_0052; K_0543_0062); imprisoned because of adultery with an Upadhyānī Bāhunī in 1916 (VS 1973, K_0168_0003); replaced as abbot by Paramahaṃsanātha in 1916 (VS 1973, K_0168_0001)."@ne ;
    rdfs:seeAlso nepalica_reg:117 ;
    foaf:name "Dhārīnātha"@ne ;
    gndo:surname "Nātha"@ne .

nepalica:8637#Gauḍa_Deśa a gn:Feature ;
    rdfs:label "Gauḍa Deśa"@ne ;
    gn:name "Gauḍa Deśa"@ne ;
    rdfs:comment "a kingdom in the region of modern-day Bengal"@en ;
    rdfs:seeAlso nepalica_reg:549 .

nepalica:8637#Gaṃḍavālāl a gn:Feature ;
    rdfs:label "Gaṃḍavālāl"@ne ,
        "गंडवालाल्‌को"@ne ;
    gn:name "Gaṃḍavālāl"@ne ;
    rdfs:comment "location needs to be verified; document suggests a locality in the Kathmandu Valley."@en ;
    rdfs:seeAlso nepalica_reg:1233 ;
    skos:altLabel "Gaṃḍavāhāla"@ne ,
        "Gaṃḍavāla"@ne ,
        "Gaṃḍavīlāla"@ne .

nepalica:8637#Jayaprakāśa_Malla a foaf:Person ;
    rdfs:label "Jayaprakāśa Malla"@ne ;
    rdfs:comment "d. 1768; king of Kathmandu (r. 1736–1746, and 1750–1768);"@ne ;
    rdfs:seeAlso dbr:seond_priority_when_data_is_Null ,
        geonames:second_priority_when_data_is_Null ,
        gnd:120152622 ,
        nepalica_reg:556 ,
        viaf:8211319 ,
        wiki:Jaya_Prakash_Malla ,
        wikidata:second_priority_when_data_is_Null ;
    foaf:name "Jayaprakāśa Malla"@ne ;
    gndo:surname "Malla"@ne .

nepalica:8637#Jogīṭāra a gn:Feature ;
    rdfs:label "Jogīṭāra"@ne ,
        "जोगीटार"@ne ;
    gn:name "Jogīṭāra"@ne ;
    rdfs:comment "location needs to be verified; document suggests a field in Deurali."@en ;
    rdfs:seeAlso nepalica_reg:1239 ;
    skos:altLabel "Jogiṭāra"@ne .

nepalica:8637#Kathmandu_Valley a gn:Feature ;
    rdfs:label "Kathmandu Valley"@ne ;
    gn:name "Kathmandu Valley"@ne ;
    rdfs:comment "also known as: Nepāla, Nepālakhalaṭā, Nepālamaṇḍala, Nepāla Upatyakā; details: a bowl-shaped valley of 665 square km with a lower altitude of 1,425 metres (4,675 ft) above sea level consisting of the areas of Kathmandu, Patan, Bhaktapur, Kirtipur and Thimi and a number of smaller municipalities; normdata:"@en ;
    rdfs:seeAlso gnd:4030037-7 ,
        nepalica_reg:113 ,
        viaf:315526926 ,
        wiki:Kathmandu_Valley .

nepalica:8637#Kiṃḍol a gn:Feature ;
    rdfs:label "Kiṃḍol"@ne ,
        "कींडोल्‌को"@ne ;
    gn:name "Kiṃḍol"@ne ;
    rdfs:comment "a locality west of Svayambhunātha."@en ;
    rdfs:seeAlso nepalica_reg:566 ;
    skos:altLabel "Kimaḍola"@ne .

nepalica:8637#Koṣayanāk a gn:Feature ;
    rdfs:label "Koṣayanāk"@ne ,
        "कोषयना"@ne ;
    gn:name "Koṣayanāk"@ne ;
    rdfs:comment "location needs to be verified; document suggests a locality in the Kathmandu Valley."@en ;
    rdfs:seeAlso nepalica_reg:1235 ;
    skos:altLabel "Koṣayanāka"@ne ,
        "Koṣaṣanāka"@ne .

nepalica:8637#Kvāṭha a gn:Feature ;
    rdfs:label "Kvāṭha"@ne ,
        "क्वाठछेउको"@ne ;
    gn:name "Kvāṭha"@ne ;
    rdfs:comment "location needs to be verified; document suggests a locality in the Kathmandu Valley."@en ;
    rdfs:seeAlso nepalica_reg:1244 ;
    skos:altLabel "Kvāṭa"@ne .

nepalica:8637#Kāntīpura a gn:Feature ;
    rdfs:label "Kāntīpura"@ne ,
        "कांतीपुर"@ne ;
    gn:name "Kāntīpura"@ne ;
    rdfs:comment "also known as: Kāḍamāḍau, Kantipur, Kāṣthamaṇḍapa, Kāṭhamāḍau, Kāṭhmāḍu, Yẽ; capital of Nepal, declared capital by Pṛthvīnārāyaṇa Śāha on 21 March 1770; a district in Central Nepal, part of Bagmati Province;"@en ;
    rdfs:seeAlso dbr:Kathmandu ,
        geonames:12095484 ,
        geonames:1283240 ,
        gnd:4030036-5 ,
        nepalica_reg:26 ,
        viaf:158284130 ,
        wiki:Kathmandu ,
        wiki:Kathmandu_District ,
        wikidata:testont_wikidata_1232 ;
    skos:altLabel "Kathmandu"@ne .

nepalica:8637#Lapaṭṭecokoṭ a gn:Feature ;
    rdfs:label "Lapaṭṭecokoṭ"@ne ,
        "लपट्टेचोकोट्‌को"@ne ;
    gn:name "Lapaṭṭecokoṭ"@ne ;
    rdfs:comment "location needs to be verified; document suggests a locality in the Kathmandu Valley."@en ;
    rdfs:seeAlso nepalica_reg:1226 ;
    skos:altLabel "Lapaṭyaco Koṭa"@ne ,
        "Lapaṭyecokoṭ"@ne .

nepalica:8637#Molapāku a gn:Feature ;
    rdfs:label "Molapāku"@ne ,
        "मोलपाकुको"@ne ;
    gn:name "Molapāku"@ne ;
    rdfs:comment "location needs to be verified; document suggests a locality in the Kathmandu Valley."@en ;
    rdfs:seeAlso nepalica_reg:1217 .

nepalica:8637#Molapāku_Nadīvārī_(°_Nadivāri) a gn:Feature ;
    rdfs:label "Molapāku Nadīvārī (° Nadivāri)"@ne ,
        "मोलपाकु नदीवारीको"@ne ;
    gn:name "Molapāku Nadīvārī (° Nadivāri)"@ne ;
    rdfs:comment "location needs to be verified; document suggests a locality in the Kathmandu Valley."@en ;
    rdfs:seeAlso nepalica_reg:1218 .

nepalica:8637#Māla a gn:Feature ;
    rdfs:label "Māla"@ne ,
        "मालको"@ne ;
    gn:name "Māla"@ne ;
    rdfs:comment "location needs to be verified; document suggests a locality in the Kathmandu Valley."@en ;
    rdfs:seeAlso nepalica_reg:1223 .

nepalica:8637#Mṛgasthalī a gn:Feature ;
    rdfs:label "Mṛgasthalī"@ne ;
    gn:name "Mṛgasthalī"@ne ;
    rdfs:comment "a forest located between the Paśupatinātha temple and the Guhyeśvarī Temple in Deopatan; seat of a monastery of the Nātha tradition; list of mahantas (cf. Naraharinātha n.d.: 123-124; for Naraharinātha and his successors, see Anonymous VS 2074: ta-tha): ... Chāyānātha Guhānātha Kṛpānātha Kamalanātha Jvālānātha Māyānātha Siddhanātha Buddhinātha Prayoganātha Bālakanātha Hukaṃnātha Haṃsanātha (VS 1933-"@en ;
    rdfs:seeAlso nepalica_reg:119 .

nepalica:8637#Nārāṃnātha_Jogī a foaf:Person ;
    rdfs:label "Nārāṃnātha Jogī"@ne ;
    rdfs:comment "Also Nārāṃnātha Jogī. A nāthayogī. A number of document copies are assented to by him as abbot (pīra or pīrajī) probably of the Mṛgasthalī monastery (cf. K 44/56; K 451/56-59). Date uncertain (but after 1876 (VS 1933))"@ne ;
    rdfs:seeAlso nepalica_reg:130 ;
    foaf:name "Nārāṃnātha Jogī"@ne ;
    gndo:surname "Nātha"@ne .

nepalica:8637#Ogla_Ṭola a gn:Feature ;
    rdfs:label "Ogla Ṭola"@ne ;
    gn:name "Ogla Ṭola"@ne ;
    rdfs:comment "also known as Vāghaḥ (Toffin 1994: 451–452, 454); a city quarter (ṭola) in upper Kathmandu around Indracoka."@en ;
    rdfs:seeAlso nepalica_reg:1142 .

nepalica:8637#Patan a gn:Feature ;
    rdfs:label "Patan"@ne ;
    gn:name "Patan"@ne ;
    rdfs:comment "also known as Lalitpur, Lalitapura; one of the three major cities in the Kathmandu Valley; a district in Central Nepal, part of the Bagmati Province;  _Nepal."@en ;
    rdfs:seeAlso dbr:Lalitpur ,
        nepalica_reg:27 ,
        wiki:Lalitpur,Nepal .

nepalica:8637#Paṃbhu a gn:Feature ;
    rdfs:label "Paṃbhu"@ne ,
        "पंभुछेउको"@ne ;
    gn:name "Paṃbhu"@ne ;
    rdfs:comment "location needs to be verified; document suggests a locality in the Kathmandu Valley."@en ;
    rdfs:seeAlso nepalica_reg:1236 .

nepalica:8637#Paṇḍu a foaf:Person ;
    rdfs:label "Paṇḍu"@ne ,
        "पंडुव्राह्मणको"@ne ;
    schema:gender schema:Male ;
    rdfs:comment "died: before 1769;  details: a brahmin."@ne ;
    rdfs:seeAlso nepalica_reg:560 ;
    skos:altLabel "Paṃḍu" ;
    foaf:name "Paṇḍu"@ne ;
    gndo:surname ""@ne .

nepalica:8637#Phīva a gn:Feature ;
    rdfs:label "Phīva"@ne ,
        "फीवछेउको"@ne ;
    gn:name "Phīva"@ne ;
    rdfs:comment "location needs to be verified; document suggests a locality in the Kathmandu Valley."@en ;
    rdfs:seeAlso nepalica_reg:1228 .

nepalica:8637#Puḍopā a gn:Feature ;
    rdfs:label "Puḍopā"@ne ,
        "पुडोपाको"@ne ;
    gn:name "Puḍopā"@ne ;
    rdfs:comment "location needs to be verified; document suggests a locality in the Kathmandu Valley."@en ;
    rdfs:seeAlso nepalica_reg:1225 ;
    skos:altLabel "Puḍoṃpā"@ne .

nepalica:8637#Pāpīgāu a gn:Feature ;
    rdfs:label "Pāpīgāu"@ne ,
        "पापीगाउको"@ne ;
    gn:name "Pāpīgāu"@ne ;
    rdfs:comment "location needs to be verified; document suggests a locality in the Kathmandu Valley."@en ;
    rdfs:seeAlso nepalica_reg:1234 ;
    skos:altLabel "Pāpigāũ"@ne ,
        "Pāpīgāū"@ne .

nepalica:8637#Pṛthvīnārāyaṇa_Śāha a foaf:Person ;
    rdfs:label "Pṛthvīnārāyaṇa Śāha"@ne ;
    schema:gender schema:Male ;
    rdfs:comment "born: 1720 at Gorkha; died: 11 January 1775 at Devighat;  father: Narabhūpāla Śāha, king of Gorkha; spouse: Indra Kumārī Devī, Narendra Rājyalakṣmī Devī; children: Pratāpa Siṃha Śāha, Bahādura Śāha, Vilāsa Kumārī Śāha; details: king of Gorkha (r. 3 April 1743–1768); king of Nepal (r. 1768-1775); normdata:"@ne ;
    rdfs:seeAlso dbr:Prithvi_Narayan_Sha ,
        gnd:119173816 ,
        nepalica_reg:178 ,
        viaf:5735314 ,
        wiki:Prithvi_Narayan_Shah ,
        wikidata:second_priority_when_data_is_Null ;
    foaf:name "Pṛthvīnārāyaṇa Śāha"@ne ;
    gndo:surname "Śāha"@ne .

nepalica:8637#Raṣuvu a gn:Feature ;
    rdfs:label "Raṣuvu"@ne ,
        "रषुवुछेउको"@ne ;
    gn:name "Raṣuvu"@ne ;
    rdfs:comment "location needs to be verified; document suggests a locality in the Kathmandu Valley."@en ;
    rdfs:seeAlso nepalica_reg:1247 .

nepalica:8637#Syāṃpurī a gn:Feature ;
    rdfs:label "Syāṃpurī"@ne ,
        "डीहीछेउको"@ne ;
    gn:name "Syāṃpurī"@ne ;
    rdfs:comment "location needs to be verified; document suggests a locality in the Kathmandu Valley."@en ;
    rdfs:seeAlso nepalica_reg:1245 ;
    skos:altLabel "Syāmapuri"@ne ,
        "Syāmpurī"@ne ,
        "Syāṃpuri"@ne .

nepalica:8637#Sāṃlā a gn:Feature ;
    rdfs:label "Sāṃlā"@ne ,
        "सांलाछेउको"@ne ;
    gn:name "Sāṃlā"@ne ;
    rdfs:comment "also known as Sāṅlā or Sāṅglā; a village and former Village Development Committee in Kathmandu district;  _Nepal."@en ;
    rdfs:seeAlso gnd:7962433 ,
        nepalica_reg:1243 ,
        wiki:Sangla ;
    skos:altLabel "Sāṅglā"@ne ,
        "Sāṅlā"@ne .

nepalica:8637#Ta_Bahā a gn:Feature ;
    rdfs:label "Ta Bahā"@ne ;
    gn:name "Ta Bahā"@ne ;
    rdfs:comment "also known as: Taḥ Bāhāḥ; a Buddhist monastery in Patan and the city quarter (ṭola) surrounding it"@en ;
    rdfs:seeAlso nepalica_reg:567 .

nepalica:8637#Tapīṃtā a gn:Feature ;
    rdfs:label "Tapīṃtā"@ne ,
        "तपींताको"@ne ;
    gn:name "Tapīṃtā"@ne ;
    rdfs:comment "location needs to be verified; document suggests a locality in the Kathmandu Valley."@en ;
    rdfs:seeAlso nepalica_reg:1222 ;
    skos:altLabel "Tapiṃtā"@ne .

nepalica:8637#Tyapadhu a gn:Feature ;
    rdfs:label "Tyapadhu"@ne ,
        "त्यपधुछेउको"@ne ;
    gn:name "Tyapadhu"@ne ;
    rdfs:comment "location needs to be verified; document suggests a locality in the Kathmandu Valley."@en ;
    rdfs:seeAlso nepalica_reg:1238 ;
    skos:altLabel "Tyapadhuka"@ne .

nepalica:8637#Vaṃsī a gn:Feature ;
    rdfs:label "Vaṃsī"@ne ,
        "वंसीको"@ne ;
    gn:name "Vaṃsī"@ne ;
    rdfs:comment "location needs to be verified; document suggests a locality in the Kathmandu Valley."@en ;
    rdfs:seeAlso dbr:testont_dbr_1232 ,
        geonames:testont_geoname_1232 ,
        gnd:testont_gnd_1232 ,
        nepalica_reg:1232 ,
        viaf:testont_viaf_1232 ,
        wiki:testont_wiki_1232 ,
        wikidata:testont_wikidata_1232 ;
    skos:altLabel "Vaṃsi"@ne ,
        "Vā̃sī"@ne .

nepalica:8637#Vaṃṣuḍola a gn:Feature ;
    rdfs:label "Vaṃṣuḍola"@ne ,
        "वंषुडोलको"@ne ;
    gn:name "Vaṃṣuḍola"@ne ;
    rdfs:comment "location needs to be verified; document suggests a locality in the Kathmandu Valley."@en ;
    rdfs:seeAlso nepalica_reg:1231 ;
    skos:altLabel "Vaṣuḍol"@ne .

nepalica:8637#Veṣāvu a gn:Feature ;
    rdfs:label "Veṣāvu"@ne ,
        "वेषावुको"@ne ;
    gn:name "Veṣāvu"@ne ;
    rdfs:comment "location needs to be verified; document suggests a locality in the Kathmandu Valley."@en ;
    rdfs:seeAlso nepalica_reg:1230 .

nepalica:8637#Voṣīmāhā a gn:Feature ;
    rdfs:label "Voṣīmāhā"@ne ,
        "व"@ne ;
    gn:name "Voṣīmāhā"@ne ;
    rdfs:comment "location needs to be verified; document suggests a locality in the Kathmandu Valley."@en ;
    rdfs:seeAlso nepalica_reg:1220 ;
    skos:altLabel "Voṣimahā"@ne .

nepalica:8637#akṣara a skos:Concept ;
    rdfs:comment "[S.] n. letter of the alphabet; syllable. t.t."@en ;
    skos:prefLabel "akṣara"@ne ;
    skos:related nepalica_gloss:2631 .

nepalica:8637#aputālī a skos:Concept ;
    rdfs:comment "var. aputāli; also maryo aputālī / moroaputālī; n. escheatable property that falls to the state if a person dies without heirs. t.t."@en ;
    skos:prefLabel "aputālī"@ne ;
    skos:related dbr:testword_dbr_2629 ,
        nepalica_gloss:2629 ,
        wiki:testword_wiki_2629 ,
        wikidata:testword_wikidata_2629 .

nepalica:8637#cakrapūjā a skos:Concept ;
    rdfs:comment "[S.] var. cakrapujā; n. lit. \"worship in a circle\", a ritual performed by the Kanphaṭṭās in an annual cycle in different localities in Kathmandu Valley (see Unbescheid 1980: 109-127 and passim). t.t."@en ;
    skos:prefLabel "cakrapūjā"@ne ;
    skos:related nepalica_gloss:2002 .

nepalica:8637#cula a skos:Concept ;
    rdfs:comment "var. cul, cura, cu; n. unit of land measurement, one fourth of a ropanī or khā. t.t."@en ;
    skos:prefLabel "cula"@ne ;
    skos:related nepalica_gloss:2628 .

nepalica:8637#ghaṭasthāpana a skos:Concept ;
    rdfs:comment "[S.] n. lit. \"setting up the jar\", a ritual that marks the beginning of the Navarātra festival. t.t."@en ;
    skos:prefLabel "ghaṭasthāpana"@ne ;
    skos:related nepalica_gloss:2657 .

nepalica:8637#guṭha a skos:Concept ;
    rdfs:comment "[fr. S. goṣṭhī] var. guṭh, guthi; n. 1) a socio-religious organization that manages and finances religious and charitable functions, a trust. 2) “endowed lands or other sources of revenue for financing religious and charitable functions“ (M.R. Pant 2002: 132; cf. M.C. Regmi 1988: 267). t.t."@en ;
    skos:altLabel "guṭhī"@ne ;
    skos:prefLabel "guṭha"@ne ;
    skos:related dbr:testword_dbr_932 ,
        geonames:testword_geonames_932 ,
        gnd:testword_gnd_932 ,
        nepalica_gloss:932 ,
        viaf:testword_viaf_932 ,
        wiki:testword_wiki_932 ,
        wikidata:testword_wikidata_932 .

nepalica:8637#kavīndramallī_ṭaṃkā a skos:Concept ;
    rdfs:comment "n. a coin circulated by Pratāpa Malla; often abbreviated as kaṭaṃ. t.t."@en ;
    skos:prefLabel "kavīndramallī ṭaṃkā"@ne ;
    skos:related nepalica_gloss:2645 .

nepalica:8637#kheta a skos:Concept ;
    rdfs:comment "[fr. S. kṣetra] var. khet, kheṭ; n. 1) irrigated land in the hill region suitable for the cultivation of rice and wheat. 2) a measure of land in the hill region equal to 25 ropanīs or 100 murīs (ca. 1.25 hectares) (M.C. Regmi 1999: 136-137 ; cf. M.C. Regmi 1999: 234 ; M.C. Regmi 1978: 162 ; M.C. Regmi 1978: 227 ; M.C. Regmi 1978: 860 ; M.C. Regmi 1995: 77; Adhikari 1984: 351; M.R. Pant 2002: 133; Whelpton 1991: 284 ). t.t."@en ;
    skos:prefLabel "kheta"@ne ;
    skos:related nepalica_gloss:1957 .

nepalica:8637#kuta a skos:Concept ;
    rdfs:comment "var. kut; n. a system of tenancy under which a cultivator paid a fixed quantity of produce or a fixed amount of money as rent to the owner of the field. t.t."@en ;
    skos:prefLabel "kuta"@ne ;
    skos:related nepalica_gloss:2504 .

nepalica:8637#lālamohara a skos:Concept ;
    rdfs:comment "var. lālmohara, lālamohar, lālmohora; abbreviated mohara; n. royal document bearing the red seal. t.t."@en ;
    skos:prefLabel "lālamohara"@ne ;
    skos:related nepalica_gloss:992 .

nepalica:8637#murī a skos:Concept ;
    rdfs:comment "n. 1) also khetamuri; unit of land measurement in the hill region, comprising 1/4 ropanī with 100 muris in 1 kheta. The area varied according to the grade: 1190 sq. ft. for lands of the best grade, and 1339 sq. ft., 1487 sq. ft., and 1785 sq. ft. for lands of inferior grades. 2) volumetric unit comprising 20 pāthis (with 8 mānas to a pāthi), equivalent to 90.919 (M.R. Pant 2002: 134 ) or 87.23 (Pant and Pierce 1989: 93) liters. (M.C. Regmi 1978: 163; M.C. Regmi 1999: 235 ; M.C. Regmi 1978a: 228 ; M.C. Regmi 1978b: 862 ; Adhikari 1984: 354; M.C. Regmi 1988: 269). t.t."@en ;
    skos:prefLabel "murī"@ne ;
    skos:related nepalica_gloss:1045 .

nepalica:8637#pīramahanta a skos:Concept ;
    rdfs:comment "[P. pīra + S. mahanta] var. pīramahaṃta; n. (esp. in the Nātha tradition) title of the head of a monastery (maṭha), esp. a pañcāyātī maṭha (cf. Bouillier 2017: 60 and passim). t.t."@en ;
    skos:prefLabel "pīramahanta"@ne ;
    skos:related dbr:Abbot_(Buddhism) ,
        geonames:testword_geonames_2644 ,
        gnd:testword_gnd_2644 ,
        nepalica_gloss:2644 ,
        viaf:testword_viaf_2644 ,
        wiki:Abbot_(Buddhism) ,
        wikidata:Q1135621 .

nepalica:8637#ropanī a skos:Concept ;
    rdfs:comment "[fr. S.] var. ropani; n. unit of land measurement in the hill region, including the Kathmandu Valley, comprising four murīs. The area may vary according to the grade, but current standard area for a ropanī comprises 5,476 square feet (cf. M.C. Regmi 1999: 235 ; M.C. Regmi 1978: 864; Whelpton 1991: 286; M.C. Regmi 1995: 77; M.C. Regmi 1978: 163; M.C. Regmi 1988: 270). t.t."@en ;
    skos:prefLabel "ropanī"@ne ;
    skos:related nepalica_gloss:2051 .

nepalica:8637#tulādhāra a skos:Concept ;
    rdfs:comment "[S.] n. a Newar Buddhist subcaste of the Urāy. t.t."@en ;
    skos:prefLabel "tulādhāra"@ne ;
    skos:related nepalica_gloss:2647 .

nepalica:8637#virāma a skos:Concept ;
    rdfs:comment "[S.] var. virām; n. a diacritic mark placed below a consonant to suppress the inherent vowel that otherwise occurs with every consonant letter. t.t."@en ;
    skos:prefLabel "virāma"@ne ;
    skos:related nepalica_gloss:2630 .

nepalica:8637#Āge a skos:Concept ;
    rdfs:comment "[fr. S. agre] adv. lit. \"henceforeward\" (Riccardi 1976: 150 n. 6), especially used in administrative and legal documents to mark the beginning of a text or paragraph. In its function it is similar to uprānta. t.t."@en ;
    skos:prefLabel "Āge"@ne ;
    skos:related nepalica_gloss:2017 .

nepalica:8637#Īcaḍol a gn:Feature ;
    rdfs:label "Īcaḍol"@ne ,
        "ईचाडोलको"@ne ;
    gn:name "Īcaḍol"@ne ;
    rdfs:comment "location needs to be verified; document suggests a locality in the Kathmandu Valley."@en ;
    rdfs:seeAlso nepalica_reg:1219 ;
    skos:altLabel "Icāḍola"@ne .

nepalica:8637#Īndracok a gn:Feature ;
    rdfs:label "Īndracok"@ne ,
        "ईन्द्रचोक्‌को"@ne ;
    gn:name "Īndracok"@ne ;
    rdfs:comment "also known as: Indrachok; a central market square in Kathmandu and the area surrounding it (see also Ogla Ṭola)"@en ;
    rdfs:seeAlso dbr:Indrachok,_Kathmandu ,
        nepalica_reg:551 ,
        wiki:Indrachok,_Kathmandu ,
        wikidata:tQ2913856 ;
    skos:altLabel "Indracoka"@ne ,
        "Iṃdracoka"@ne .

nepalica:8637#Īḍā a gn:Feature ;
    rdfs:label "Īḍā"@ne ;
    gn:name "Īḍā"@ne ;
    rdfs:comment "location needs to be verified; document suggests a locality in the Kathmandu Valley."@en ;
    rdfs:seeAlso nepalica_reg:1227 ;
    skos:altLabel "Iṃḍā"@ne ,
        "Īdā"@ne ,
        "Īuḍā"@ne .

nepalica:8637#Śrī a skos:Concept ;
    rdfs:comment "[S.] n. word of blessing, can be used as apprecatio, in which case it means 'good fortune' (Pant and Pierce 1989: 12), can be used as a prefix to names of persons and gods, in which case it means 'venerable' or 'glorious' respectively. The number of śrīs used varies, depending on context. t.t."@en ;
    skos:prefLabel "Śrī"@ne ;
    skos:related nepalica_gloss:1869 .

nepalica:8637#Śrīnivāsa_Malla a foaf:Person ;
    rdfs:label "Śrīnivāsa Malla"@ne ;
    rdfs:comment "king of Patan (r. 1661–1685). normdata: wiki: Srinivasa_Malla"@ne ;
    rdfs:seeAlso nepalica_reg:552 ;
    foaf:name "Śrīnivāsa Malla"@ne ;
    gndo:surname "Malla"@ne .

nepalica:8637#Ṭaugāl a gn:Feature ;
    rdfs:label "टौगाल्‌को"@ne ,
        "Ṭaugāl"@ne ;
    gn:name "Ṭaugāl"@ne ;
    rdfs:comment "location needs to be verified; document suggests a locality in the Kathmandu Valley."@en ;
    rdfs:seeAlso nepalica_reg:1240 ;
    skos:altLabel "Ṭaugāla"@ne .

nepalica:8637#Ṭauḍhī_Josī a foaf:Person ;
    rdfs:label "ठौढी जोसीको"@ne ,
        "Ṭauḍhī Josī"@ne ;
    schema:gender schema:Male ;
    rdfs:comment "died: before 1769;  details: owned a house in Indracoka."@ne ;
    rdfs:seeAlso nepalica_reg:561 ;
    skos:altLabel "Ṭauḍhi Josi" ;
    foaf:name "Ṭauḍhī Josī"@ne ;
    gndo:surname "Josī"@ne .

nepalica:8637#Ṭepadhu a gn:Feature ;
    rdfs:label "टेपधुको"@ne ,
        "Ṭepadhu"@ne ;
    gn:name "Ṭepadhu"@ne ;
    rdfs:comment "location needs to be verified; document suggests a locality in the Kathmandu Valley."@en ;
    rdfs:seeAlso nepalica_reg:1229 .

nepalica:8637#Ṭhavailī a gn:Feature ;
    rdfs:label "ठवैलीको"@ne ,
        "Ṭhavailī"@ne ;
    gn:name "Ṭhavailī"@ne ;
    rdfs:comment "location needs to be verified; document suggests a locality in the Kathmandu Valley."@en ;
    rdfs:seeAlso nepalica_reg:1224 ;
    skos:altLabel "Vaili"@ne ,
        "Ṭhavela"@ne .

nepalica:8637#Ṭoṣa a gn:Feature ;
    rdfs:label "टोषाछेउको"@ne ,
        "Ṭoṣa"@ne ;
    gn:name "Ṭoṣa"@ne ;
    rdfs:comment "location needs to be verified; document suggests a locality in the Kathmandu Valley."@en ;
    rdfs:seeAlso dbr:testont_dbr_1241 ,
        geonames:testont_geoname_1241 ,
        gnd:testont_gnd_1241 ,
        nepalica_reg:1241 ,
        viaf:testont_viaf_1241 ,
        wiki:testont_wiki_1241 ,
        wikidata:testont_wikidata_1241 .

nepalica:8637#Ṭukucā a gn:Feature ;
    rdfs:label "टुकुचाछेउको"@ne ,
        "Ṭukucā"@ne ;
    gn:name "Ṭukucā"@ne ;
    rdfs:comment "location needs to be verified; document suggests a locality in the Kathmandu Valley."@en ;
    rdfs:seeAlso nepalica_reg:1246 .

nepalica:8637#Ṭāyemaḍu_Ṭola a gn:Feature ;
    rdfs:label "टायेमडुटोलको"@ne ,
        "Ṭāyemaḍu Ṭola"@ne ;
    gn:name "Ṭāyemaḍu Ṭola"@ne ;
    rdfs:comment "Newari name for Bangemudha (Bāṅgemuḍhā); a city quarter (ṭola) in Kathmandu"@en ;
    rdfs:seeAlso nepalica_reg:521 ;
    skos:altLabel "Thāya°"@ne ,
        "Ṭhāyemaḍu Ṭola"@ne ,
        "Ṭāyamaḍu Ṭola"@ne ,
        "Ṭāyamaḍu Ṭola or ° Ṭol"@ne .

